Got it, let's start by understanding the first part: deriving the logistic function from the log-odds. The user's notes show the steps for logit to probability, so let's go through that carefully. Then, we need to cover expected value, variance, and normal distribution properties. Let's break it down.


### Part 1: Simplifying the Logistic Regression Probability (Logit to Probability)
The logit function is defined as the natural log of the odds:  
$$ \log\left( \frac{p}{1-p} \right) = \beta_0 + \beta_1 X_1 + \dots + \beta_n X_n $$  

Let's denote the linear predictor as $\eta = \beta_0 + \beta_1 X_1 + \dots + \beta_n X_n$. So:  
$$ \log\left( \frac{p}{1-p} \right) = \eta $$  

**Step 1: Exponentiate both sides** to eliminate the log:  
$$ \frac{p}{1-p} = e^\eta $$  

**Step 2: Solve for $p$**. Multiply both sides by $(1-p)$:  
$$ p = e^\eta (1 - p) $$  

**Step 3: Expand the right-hand side**  
$$ p = e^\eta - p e^\eta $$  

**Step 4: Collect terms with $p$** on the left:  
$$ p + p e^\eta = e^\eta $$  

**Step 5: Factor out $p$** on the left:  
$$ p(1 + e^\eta) = e^\eta $$  

**Step 6: Divide both sides by $(1 + e^\eta)$** to solve for $p$:  
$$ p = \frac{e^\eta}{1 + e^\eta} $$  

We can also write this as:  
$$ p = \frac{1}{1 + e^{-\eta}} $$  
(by dividing numerator and denominator by $e^\eta$: $\frac{e^\eta}{1 + e^\eta} = \frac{1}{e^{-\eta} + 1} = \frac{1}{1 + e^{-\eta}}$)  


### Part 2: Expected Value (Mean) - Mathematical Properties
The **expected value** (or mean) of a random variable $X$ is a measure of central tendency. Let's define it for discrete and continuous cases.  

#### Discrete Random Variable  
If $X$ is discrete with possible values $x_1, x_2, \dots, x_k$ and probabilities $P(X = x_i) = p_i$, then:  
$$ \mathbb{E}[X] = \sum_{i=1}^k x_i p_i $$  

#### Continuous Random Variable  
If $X$ is continuous with probability density function (pdf) $f(x)$, then:  
$$ \mathbb{E}[X] = \int_{-\infty}^{\infty} x f(x) \, dx $$  

**Key Properties of Expected Value**:  
1. **Linearity**: For constants $a, b$ and random variables $X, Y$:  
   $$ \mathbb{E}[aX + bY] = a\mathbb{E}[X] + b\mathbb{E}[Y] $$  
   *Proof (discrete example)*:  
   $$ \mathbb{E}[aX + bY] = \sum (a x_i + b y_j) P(X=x_i, Y=y_j) = a \sum x_i P(X=x_i) + b \sum y_j P(Y=y_j) = a\mathbb{E}[X] + b\mathbb{E}[Y] $$  

2. **Constant Multiple**: $\mathbb{E}[aX] = a\mathbb{E}[X]$ (set $b=0$ in linearity).  

3. **Constant Term**: $\mathbb{E}[a] = a$ (since $P(X=a)=1$, so $\sum a \cdot 1 = a$).  


### Part 3: Variance - Mathematical Properties
The **variance** of a random variable $X$ measures spread: $\text{Var}(X) = \mathbb{E}[(X - \mathbb{E}[X])^2]$.  

#### Alternative Formula  
$$ \text{Var}(X) = \mathbb{E}[X^2] - (\mathbb{E}[X])^2 $$  
*Derivation*:  
Expand $(X - \mu)^2$ where $\mu = \mathbb{E}[X]$:  
$$ (X - \mu)^2 = X^2 - 2\mu X + \mu^2 $$  
Take expectation:  
$$ \mathbb{E}[(X - \mu)^2] = \mathbb{E}[X^2] - 2\mu \mathbb{E}[X] + \mu^2 = \mathbb{E}[X^2] - 2\mu^2 + \mu^2 = \mathbb{E}[X^2] - \mu^2 $$  


**Key Properties of Variance**:  
1. **Constant Term**: $\text{Var}(a) = 0$ (since $(a - a)^2 = 0$, so expectation is 0).  

2. **Constant Multiple**: $\text{Var}(aX) = a^2 \text{Var}(X)$  
   *Derivation*:  
   $$ \text{Var}(aX) = \mathbb{E}[(aX - \mathbb{E}[aX])^2] = \mathbb{E}[(aX - a\mu)^2] = \mathbb{E}[a^2(X - \mu)^2] = a^2 \mathbb{E}[(X - \mu)^2] = a^2 \text{Var}(X) $$  

3. **Independent Variables**: If $X$ and $Y$ are independent, then $\text{Var}(X + Y) = \text{Var}(X) + \text{Var}(Y)$  
   *Derivation*:  
   $$ \text{Var}(X + Y) = \mathbb{E}[(X + Y - \mathbb{E}[X+Y])^2] = \mathbb{E}[(X - \mu_X + Y - \mu_Y)^2] $$  
   Expand:  
   $$ = \mathbb{E}[(X - \mu_X)^2 + 2(X - \mu_X)(Y - \mu_Y) + (Y - \mu_Y)^2] $$  
   Since $X, Y$ are independent, $\mathbb{E}[(X - \mu_X)(Y - \mu_Y)] = \mathbb{E}[X - \mu_X]\mathbb{E}[Y - \mu_Y] = 0 \cdot 0 = 0$  
   Thus:  
   $$ = \mathbb{E}[(X - \mu_X)^2] + \mathbb{E}[(Y - \mu_Y)^2] = \text{Var}(X) + \text{Var}(Y) $$  


### Part 4: Normal Distribution - Properties
The **normal distribution** (Gaussian distribution) for a random variable $X$ with mean $\mu$ and variance $\sigma^2$ has pdf:  
$$ f(x) = \frac{1}{\sigma \sqrt{2\pi}} e^{-\frac{(x - \mu)^2}{2\sigma^2}}, \quad x \in \mathbb{R} $$  


#### 1. Mean of Normal Distribution  
To find $\mathbb{E}[X]$ for $X \sim \mathcal{N}(\mu, \sigma^2)$:  
$$ \mathbb{E}[X] = \int_{-\infty}^{\infty} x \cdot \frac{1}{\sigma \sqrt{2\pi}} e^{-\frac{(x - \mu)^2}{2\sigma^2}} \, dx $$  
Let $z = \frac{x - \mu}{\sigma}$, so $x = \mu + \sigma z$, $dx = \sigma dz$. Substitute:  
$$ \mathbb{E}[X] = \int_{-\infty}^{\infty} (\mu + \sigma z) \cdot \frac{1}{\sigma \sqrt{2\pi}} e^{-\frac{z^2}{2}} \cdot \sigma dz = \int_{-\infty}^{\infty} (\mu + \sigma z) \cdot \frac{1}{\sqrt{2\pi}} e^{-\frac{z^2}{2}} dz $$  
Split the integral:  
$$ = \mu \int_{-\infty}^{\infty} \frac{1}{\sqrt{2\pi}} e^{-\frac{z^2}{2}} dz + \sigma \int_{-\infty}^{\infty} z \cdot \frac{1}{\sqrt{2\pi}} e^{-\frac{z^2}{2}} dz $$  
The first integral is 1 (integral of standard normal pdf). The second integral is 0 (odd function over symmetric interval). Thus:  
$$ \mathbb{E}[X] = \mu \cdot 1 + \sigma \cdot 0 = \mu $$  


#### 2. Variance of Normal Distribution  
To find $\text{Var}(X) = \mathbb{E}[(X - \mu)^2]$:  
$$ \text{Var}(X) = \int_{-\infty}^{\infty} (x - \mu)^2 \cdot \frac{1}{\sigma \sqrt{2\pi}} e^{-\frac{(x - \mu)^2}{2\sigma^2}} \, dx $$  
Let $z = \frac{x - \mu}{\sigma}$, so $(x - \mu)^2 = \sigma^2 z^2$, $dx = \sigma dz$. Substitute:  
$$ \text{Var}(X) = \int_{-\infty}^{\infty} \sigma^2 z^2 \cdot \frac{1}{\sigma \sqrt{2\pi}} e^{-\frac{z^2}{2}} \cdot \sigma dz = \sigma^2 \int_{-\infty}^{\infty} z^2 \cdot \frac{1}{\sqrt{2\pi}} e^{-\frac{z^2}{2}} dz $$  
The integral $\int_{-\infty}^{\infty} z^2 \phi(z) dz$ (where $\phi(z)$ is standard normal pdf) is known to be 1 (since variance of standard normal is 1). Thus:  
$$ \text{Var}(X) = \sigma^2 \cdot 1 = \sigma^2 $$  


#### 3. Moment Generating Function (MGF) of Normal Distribution  
The MGF of $X \sim \mathcal{N}(\mu, \sigma^2)$ is $M_X(t) = \mathbb{E}[e^{tX}]$.  
$$ M_X(t) = \int_{-\infty}^{\infty} e^{tx} \cdot \frac{1}{\sigma \sqrt{2\pi}} e^{-\frac{(x - \mu)^2}{2\sigma^2}} dx $$  
Complete the square in the exponent:  
$$ tx - \frac{(x - \mu)^2}{2\sigma^2} = -\frac{1}{2\sigma^2} \left( x^2 - 2\mu x + \mu^2 - 2\sigma^2 t x \right) = -\frac{1}{2\sigma^2} \left( x^2 - 2(\mu + \sigma^2 t)x + \mu^2 \right) $$  
Complete the square for $x$:  
$$ = -\frac{1}{2\sigma^2} \left( (x - (\mu + \sigma^2 t))^2 - (\mu + \sigma^2 t)^2 + \mu^2 \right) = -\frac{1}{2\sigma^2} (x - (\mu + \sigma^2 t))^2 + \frac{2\mu \sigma^2 t + \sigma^4 t^2}{2\sigma^2} $$  
Simplify the exponent:  
$$ = -\frac{1}{2\sigma^2} (x - (\mu + \sigma^2 t))^2 + \mu t + \frac{\sigma^2 t^2}{2} $$  
Thus, the integral becomes:  
$$ M_X(t) = e^{\mu t + \frac{\sigma^2 t^2}{2}} \int_{-\infty}^{\infty} \frac{1}{\sigma \sqrt{2\pi}} e^{-\frac{(x - (\mu + \sigma^2 t))^2}{2\sigma^2}} dx $$  
The integral is 1 (integral of normal pdf with mean $\mu + \sigma^2 t$ and variance $\sigma^2$). Thus:  
$$ M_X(t) = e^{\mu t + \frac{\sigma^2 t^2}{2}} $$  


#### 4. Linear Transformation of Normal Variables  
If $X \sim \mathcal{N}(\mu, \sigma^2)$, then $aX + b \sim \mathcal{N}(a\mu + b, a^2 \sigma^2)$.  
*Proof using MGF*:  
Let $Y = aX + b$. Then $M_Y(t) = \mathbb{E}[e^{tY}] = \mathbb{E}[e^{t(aX + b)}] = e^{tb} \mathbb{E}[e^{taX}] = e^{tb} M_X(ta)$.  
Substitute $M_X(ta) = e^{\mu (ta) + \frac{\sigma^2 (ta)^2}{2}}$:  
$$ M_Y(t) = e^{tb} \cdot e^{a \mu t + \frac{a^2 \sigma^2 t^2}{2}} = e^{(a \mu + b) t + \frac{(a \sigma)^2 t^2}{2}} $$  
Which is the MGF of $\mathcal{N}(a\mu + b, a^2 \sigma^2)$. Since MGF uniquely determines the distribution, $Y \sim \mathcal{N}(a\mu + b, a^2 \sigma^2)$.  


### Summary  
1. **Logistic Probability**: Starting from log-odds $\log\left( \frac{p}{1-p} \right) = \eta$, we derive $p = \frac{e^\eta}{1 + e^\eta}$.  

2. **Expected Value**: Defined for discrete and continuous RVs, with linearity as a key property.  

3. **Variance**: Measures spread, with properties for constants and independent variables.  

4. **Normal Distribution**: Mean $\mu$, variance $\sigma^2$, MGF $e^{\mu t + \frac{\sigma^2 t^2}{2}}$, and linear transformations preserve normality.  


Let me know if you need more detail on any specific part!To address your request, we’ll break this into two main sections: **(1) Simplifying the Logistic Regression Probability** (from log-odds to probability) and **(2) Deriving Properties of Expected Value, Variance, and the Normal Distribution**.  


### Section 1: Simplifying the Logistic Regression Probability  
Logistic regression models the **log-odds** of a binary outcome. Let’s derive the probability $p$ from the log-odds formula.  


#### Step 1: Start with the Log-Odds Definition  
The log-odds of an event (probability $p$) is defined as:  
$$ \log\left( \frac{p}{1-p} \right) = \beta_0 + \beta_1 X_1 + \dots + \beta_n X_n $$  

Let $\eta = \beta_0 + \beta_1 X_1 + \dots + \beta_n X_n$ (the “linear predictor”). Then:  
$$ \log\left( \frac{p}{1-p} \right) = \eta $$  


#### Step 2: Exponentiate Both Sides  
To eliminate the logarithm, exponentiate both sides with base $e$:  
$$ \frac{p}{1-p} = e^\eta $$  


#### Step 3: Solve for $p$  
Multiply both sides by $(1-p)$:  
$$ p = e^\eta (1 - p) $$  

Expand the right-hand side:  
$$ p = e^\eta - p e^\eta $$  

Collect terms with $p$ on the left:  
$$ p + p e^\eta = e^\eta $$  

Factor out $p$:  
$$ p \left( 1 + e^\eta \right) = e^\eta $$  

Divide both sides by $(1 + e^\eta)$:  $$ p = \frac{e^\eta}{1 + e^\eta} $$  #### Alternative Form (Optional)  
Divide numerator and denominator by $e^\eta$ to get:  
$$ p = \frac{1}{1 + e^{-\eta}} $$
### Section 2: Deriving Properties of Expected Value, Variance, and the Normal Distribution  
#### 1. Expected Value (Mean)  
The **expected value** $\mathbb{E}[X]$ measures the “central tendency” of a random variable $X$.  
##### Definition by Case:  
- **Discrete Random Variable**: If $X$ takes values $x_1, x_2, \dots, x_k$ with probabilities $P(X = x_i) = p_i$, then:  
  $$ \mathbb{E}[X] = \sum_{i=1}^k x_i \cdot p_i $$  

- **Continuous Random Variable**: If $X$ has probability density function (pdf) $f(x)$, then:  
  $$ \mathbb{E}[X] = \int_{-\infty}^{\infty} x \cdot f(x) \, dx $$  


##### Key Properties:  
- **Linearity**: For constants $a, b$ and random variables $X, Y$:  
  $$ \mathbb{E}[aX + bY] = a\mathbb{E}[X] + b\mathbb{E}[Y] $$  
  *Proof (discrete example)*:  
  $$ \mathbb{E}[aX + bY] = \sum (a x_i + b y_j) P(X=x_i, Y=y_j) = a \sum x_i P(X=x_i) + b \sum y_j P(Y=y_j) = a\mathbb{E}[X] + b\mathbb{E}[Y] $$  

- **Constant Multiple**: $\mathbb{E}[aX] = a\mathbb{E}[X]$ (set $b = 0$ in linearity).  
- **Constant Term**: $\mathbb{E}[a] = a$ (since $P(X = a) = 1$, so $\sum a \cdot 1 = a$).  


#### 2. Variance  
The **variance** $\text{Var}(X)$ measures the “spread” of a random variable. It is defined as:  
$$ \text{Var}(X) = \mathbb{E}\left[ (X - \mathbb{E}[X])^2 \right] $$  


##### Alternative Formula:  
$$ \text{Var}(X) = \mathbb{E}[X^2] - \left( \mathbb{E}[X] \right)^2 $$  
*Derivation*:  
Expand $(X - \mu)^2$ (where $\mu = \mathbb{E}[X]$):  
$$ (X - \mu)^2 = X^2 - 2\mu X + \mu^2 $$  
Take the expectation:  
$$ \mathbb{E}\left[ (X - \mu)^2 \right] = \mathbb{E}[X^2] - 2\mu \mathbb{E}[X] + \mu^2 = \mathbb{E}[X^2] - 2\mu^2 + \mu^2 = \mathbb{E}[X^2] - \mu^2 $$  


##### Key Properties:  
- **Constant Term**: $\text{Var}(a) = 0$ (since $(a - a)^2 = 0$, so $\mathbb{E}[0] = 0$).  
- **Constant Multiple**: $\text{Var}(aX) = a^2 \text{Var}(X)$  
  *Derivation*:  
  $$ \text{Var}(aX) = \mathbb{E}\left[ (aX - \mathbb{E}[aX])^2 \right] = \mathbb{E}\left[ (aX - a\mu)^2 \right] = \mathbb{E}\left[ a^2 (X - \mu)^2 \right] = a^2 \mathbb{E}\left[ (X - \mu)^2 \right] = a^2 \text{Var}(X) $$  

- **Independent Variables**: If $X$ and $Y$ are independent, then:  
  $$ \text{Var}(X + Y) = \text{Var}(X) + \text{Var}(Y) $$  
  *Derivation*:  
  Expand $\mathbb{E}\left[ (X + Y - \mathbb{E}[X+Y])^2 \right]$:  
  $$ \mathbb{E}\left[ (X - \mu_X + Y - \mu_Y)^2 \right] = \mathbb{E}\left[ (X - \mu_X)^2 + 2(X - \mu_X)(Y - \mu_Y) + (Y - \mu_Y)^2 \right] $$  
  Since $X, Y$ are independent, $\mathbb{E}\left[ (X - \mu_X)(Y - \mu_Y) \right] = 0$ (covariance of independent variables is 0). Thus:  
  $$ \text{Var}(X + Y) = \text{Var}(X) + \text{Var}(Y) $$  


#### 3. Normal Distribution  
A random variable $X$ follows a **normal distribution** $\mathcal{N}(\mu, \sigma^2)$ if its pdf is:  
$$ f(x) = \frac{1}{\sigma \sqrt{2\pi}} e^{-\frac{(x - \mu)^2}{2\sigma^2}}, \quad x \in \mathbb{R} $$  


##### 3.1 Mean of a Normal Variable  
To find $\mathbb{E}[X]$ for $X \sim \mathcal{N}(\mu, \sigma^2)$:  
$$ \mathbb{E}[X] = \int_{-\infty}^{\infty} x \cdot \frac{1}{\sigma \sqrt{2\pi}} e^{-\frac{(x - \mu)^2}{2\sigma^2}} \, dx $$  

Let $z = \frac{x - \mu}{\sigma}$ (so $x = \mu + \sigma z$, $dx = \sigma dz$). Substitute:  
$$ \mathbb{E}[X] = \int_{-\infty}^{\infty} (\mu + \sigma z) \cdot \frac{1}{\sigma \sqrt{2\pi}} e^{-\frac{z^2}{2}} \cdot \sigma dz = \int_{-\infty}^{\infty} (\mu + \sigma z) \cdot \frac{1}{\sqrt{2\pi}} e^{-\frac{z^2}{2}} dz $$  

Split the integral:  
$$ = \mu \int_{-\infty}^{\infty} \frac{1}{\sqrt{2\pi}} e^{-\frac{z^2}{2}} dz + \sigma \int_{-\infty}^{\infty} z \cdot \frac{1}{\sqrt{2\pi}} e^{-\frac{z^2}{2}} dz $$  

- The first integral equals 1 (it’s the integral of the **standard normal pdf**).  
- The second integral equals 0 (it’s an odd function integrated over a symmetric interval).  

Thus:  
$$ \mathbb{E}[X] = \mu \cdot 1 + \sigma \cdot 0 = \mu $$  


##### 3.2 Variance of a Normal Variable  
To find $\text{Var}(X) = \mathbb{E}\left[ (X - \mu)^2 \right]$:  
$$ \text{Var}(X) = \int_{-\infty}^{\infty} (x - \mu)^2 \cdot \frac{1}{\sigma \sqrt{2\pi}} e^{-\frac{(x - \mu)^2}{2\sigma^2}} \, dx $$  

Let $z = \frac{x - \mu}{\sigma}$ (so $(x - \mu)^2 = \sigma^2 z^2$, $dx = \sigma dz$). Substitute:  
$$ \text{Var}(X) = \int_{-\infty}^{\infty} \sigma^2 z^2 \cdot \frac{1}{\sigma \sqrt{2\pi}} e^{-\frac{z^2}{2}} \cdot \sigma dz = \sigma^2 \int_{-\infty}^{\infty} z^2 \cdot \frac{1}{\sqrt{2\pi}} e^{-\frac{z^2}{2}} dz $$  

The integral $\int_{-\infty}^{\infty} z^2 \cdot \frac{1}{\sqrt{2\pi}} e^{-\frac{z^2}{2}} dz = 1$ (this is the variance of the **standard normal distribution**, $\mathcal{N}(0, 1)$). Thus:  
$$ \text{Var}(X) = \sigma^2 \cdot 1 = \sigma^2 $$  


##### 3.3 Linear Transformation of Normal Variables  
If $X \sim \mathcal{N}(\mu, \sigma^2)$, then $aX + b \sim \mathcal{N}(a\mu + b, a^2 \sigma^2)$.  

*Proof (using Moment Generating Functions)*:  
The **moment generating function** (MGF) of $X$ is $M_X(t) = \mathbb{E}[e^{tX}]$. For $X \sim \mathcal{N}(\mu, \sigma^2)$, the MGF is:  
$$ M_X(t) = e^{\mu t + \frac{\sigma^2 t^2}{2}} $$  

Let $Y = aX + b$. The MGF of $Y$ is:  
$$ M_Y(t) = \mathbb{E}[e^{tY}] = \mathbb{E}[e^{t(aX + b)}] = e^{tb} \mathbb{E}[e^{taX}] = e^{tb} \cdot M_X(ta) $$  

Substitute $M_X(ta) = e^{\mu (ta) + \frac{\sigma^2 (ta)^2}{2}}$:  
$$ M_Y(t) = e^{tb} \cdot e^{a \mu t + \frac{a^2 \sigma^2 t^2}{2}} = e^{(a \mu + b) t + \frac{(a \sigma)^2 t^2}{2}} $$  

This matches the MGF of $\mathcal{N}(a\mu + b, a^2 \sigma^2)$. Since MGFs uniquely determine distributions, $Y \sim \mathcal{N}(a\mu + b, a^2 \sigma^2)$.  


### Summary  
- **Logistic Probability**: From log-odds $\log\left( \frac{p}{1-p} \right) = \eta$, we derive $p = \frac{e^\eta}{1 + e^\eta}$.  
- **Expected Value**: Measures central tendency; key property is linearity.  
- **Variance**: Measures spread; key properties include scaling by $a^2$ and additivity for independent variables.  
- **Normal Distribution**: Mean $\mu$, variance $\sigma^2$; linear transformations preserve normality.  


Let me know if you want deeper exploration of any topic!